ADT/MapLike.lean
@@ -1,0 +1,1160 @@
+/-
+Copyright (c) 2025 Amazon.com, Inc. or its affiliates. All Rights Reserved.
+Released under Apache 2.0 license as described in the file LICENSE.
+Authors: Yicheng Qian
+-/
+
+import Lean
+import ADT.List
+import ADT.OptArr
+import ADT.Logic
+import ADT.Lemmas
+import ADT.Size
+import ADT.DGetElem
+import Std.Data
+open Std
+
+/-!
+  This section defines an abstract datatype `DMapLike` and its lawful
+  counterpart `LawfulDMapLike`. An instance `inst : DMapLike γ α β` denotes
+  that `γ` models a finite, dependently typed map from `α` to `β`,
+  i.e. a function from a finite collection of elements of type `α`
+  (i.e. the keys) to `β`.
+
+  `DMapLike` is a subtype of `Membership` and `DGetElem?`. In addition,
+  it must support the following operations: `emptyWithCapacity`,
+  `insert`, `erase`, `size`
+  · `a ∈ m` iff `a` is present in the keys
+  · `emptyWithCapacity k` returns an empty map with capacity `k`.
+    The capacity parameter is present because of performance considerations.
+  · `insert m k v`: insert the key-value pair `(k, v)` to `m`. If
+    `k` is already present, its value is overriden
+  · `erase m k`: erase the key `k` from `m`
+  · `size m`: return the size of `m`
+
+  `LawfulDMapLike` specifies the behavior of the operations supported by
+  `DMapLike`, whereby the behavior of the operations are uniquely determined
+  up to `DMapLike.equiv`.
+-/
+
+section DMapLike
+
+class DMapLike (γ : Type u) (α : Type v) (β : α → Type w) extends
+  Membership α γ, DGetElem? γ α β (fun m x => x ∈ m), Size γ where
+  emptyWithCapacity {γ α β} : Nat → γ
+  insert : γ → (x : α) → (y : β x) → γ
+  erase {γ α β} : γ → α → γ
+
+def DMapLike.keyEquiv {γ₁ γ₂ α β} [inst₁ : DMapLike γ₁ α β] [inst₂ : DMapLike γ₂ α β]
+  (m₁ : γ₁) (m₂ : γ₂) := ∀ (x : α), x ∈ m₁ ↔ x ∈ m₂
+
+def DMapLike.equiv {γ₁ γ₂ α β} [inst₁ : DMapLike γ₁ α β] [inst₂ : DMapLike γ₂ α β] (m₁ : γ₁) (m₂ : γ₂) :=
+  keyEquiv (β:=β) m₁ m₂ ∧ ∀ (x : α) (h₁ : x ∈ m₁) (h₂ : x ∈ m₂), m₁[x]ᵈ'h₁ = m₂[x]ᵈ'h₂
+
+def DMapLike.equiv' {γ₁ γ₂ α β} [inst₁ : DMapLike γ₁ α β] [inst₂ : DMapLike γ₂ α β] (m₁ : γ₁) (m₂ : γ₂) :=
+  ∀ (x : α), m₁[x]ᵈ? = m₂[x]ᵈ?
+
+def DMapLike.keySubset {γ₁ γ₂ α β} [inst₁ : DMapLike γ₁ α β] [inst₂ : DMapLike γ₂ α β] (m₁ : γ₁) (m₂ : γ₂) :=
+  ∀ (x : α), x ∈ m₁ → x ∈ m₂
+
+def DMapLike.subset {γ₁ γ₂ α β} [inst₁ : DMapLike γ₁ α β] [inst₂ : DMapLike γ₂ α β] (m₁ : γ₁) (m₂ : γ₂) :=
+  ∀ (x : α) (y : β x), m₁[x]ᵈ? = .some y → m₂[x]ᵈ? =.some y
+
+theorem DMapLike.keyEquiv.refl {γ α β} [inst : DMapLike γ α β] {m : γ} : keyEquiv (β:=β) m m := by
+  simp [keyEquiv]
+
+theorem DMapLike.keyEquiv.comm {γ₁ γ₂ α β} [inst₁ : DMapLike γ₁ α β] [inst₂ : DMapLike γ₂ α β]
+  {m₁ : γ₁} {m₂ : γ₂} : keyEquiv (β:=β) m₁ m₂ ↔ keyEquiv (β:=β) m₂ m₁ := by
+  simp only [keyEquiv]
+  conv => left; enter [x]; rw [Iff.comm]
+
+theorem DMapLike.keyEquiv.symm {γ₁ γ₂ α β} [inst₁ : DMapLike γ₁ α β] [inst₂ : DMapLike γ₂ α β]
+  {m₁ : γ₁} {m₂ : γ₂} : keyEquiv (β:=β) m₁ m₂ → keyEquiv (β:=β) m₂ m₁ :=
+  DMapLike.keyEquiv.comm.mp
+
+theorem DMapLike.keyEquiv.trans {γ₁ γ₂ γ₃ α β} [inst₁ : DMapLike γ₁ α β] [inst₂ : DMapLike γ₂ α β] [inst₃ : DMapLike γ₃ α β]
+  {m₁ : γ₁} {m₂ : γ₂} {m₃ : γ₃} : keyEquiv (β:=β) m₁ m₂ → keyEquiv (β:=β) m₂ m₃ → keyEquiv (β:=β) m₁ m₃ := by
+  intro h₁ h₂ x
+  rw [h₁, h₂]
+
+theorem DMapLike.equiv.refl {γ α β} [inst : DMapLike γ α β] {m : γ} : equiv (β:=β) m m := by
+  simp [equiv, keyEquiv]
+
+theorem DMapLike.equiv.comm {γ₁ γ₂ α β} [inst₁ : DMapLike γ₁ α β] [inst₂ : DMapLike γ₂ α β]
+  {m₁ : γ₁} {m₂ : γ₂} : equiv (β:=β) m₁ m₂ ↔ equiv (β:=β) m₂ m₁ := by
+  simp only [equiv, keyEquiv.comm (m₁:=m₁)]
+  conv => enter [1, 2, x]; rw [forall_comm]
+  conv => enter [1, 2, x, h₁, h₂]; rw [Eq.comm]
+
+theorem DMapLike.equiv.symm {γ₁ γ₂ α β} [inst₁ : DMapLike γ₁ α β] [inst₂ : DMapLike γ₂ α β]
+  {m₁ : γ₁} {m₂ : γ₂} : equiv (β:=β) m₁ m₂ → equiv (β:=β) m₂ m₁ :=
+  DMapLike.equiv.comm.mp
+
+theorem DMapLike.equiv.trans {γ₁ γ₂ γ₃ α β} [inst₁ : DMapLike γ₁ α β] [inst₂ : DMapLike γ₂ α β] [inst₃ : DMapLike γ₃ α β]
+  {m₁ : γ₁} {m₂ : γ₂} {m₃ : γ₃} : equiv (β:=β) m₁ m₂ → equiv (β:=β) m₂ m₃ → equiv (β:=β) m₁ m₃ := by
+  intro h₁ h₂; apply And.intro
+  case left => intro x; rw [h₁.left, h₂.left]
+  case right =>
+    intro x h₁' h₃'
+    have h₂' := by rw [← h₂.left] at h₃'; exact h₃'
+    rw [h₁.right _ h₁' h₂', h₂.right _ h₂' h₃']
+
+theorem DMapLike.equiv'.refl {γ α β} [inst : DMapLike γ α β] {m : γ} : equiv' (β:=β) m m := by
+  simp [equiv']
+
+theorem DMapLike.equiv'.comm {γ₁ γ₂ α β} [inst₁ : DMapLike γ₁ α β] [inst₂ : DMapLike γ₂ α β]
+  {m₁ : γ₁} {m₂ : γ₂} : equiv' (β:=β) m₁ m₂ ↔ equiv' (β:=β) m₂ m₁ := by
+  simp only [equiv']
+  conv => left; enter [x]; rw [Eq.comm]
+
+theorem DMapLike.equiv'.symm {γ₁ γ₂ α β} [inst₁ : DMapLike γ₁ α β] [inst₂ : DMapLike γ₂ α β]
+  {m₁ : γ₁} {m₂ : γ₂} : equiv' (β:=β) m₁ m₂ → equiv' (β:=β) m₂ m₁ :=
+  DMapLike.equiv'.comm.mp
+
+theorem DMapLike.equiv'.trans {γ₁ γ₂ γ₃ α β} [inst₁ : DMapLike γ₁ α β] [inst₂ : DMapLike γ₂ α β] [inst₃ : DMapLike γ₃ α β]
+  {m₁ : γ₁} {m₂ : γ₂} {m₃ : γ₃} : equiv' (β:=β) m₁ m₂ → equiv' (β:=β) m₂ m₃ → equiv' (β:=β) m₁ m₃ := by
+  intro h₁ h₂ x; rw [h₁, h₂]
+
+theorem DMapLike.keyEquiv_iff_keySubset {γ₁ γ₂ α β} [inst₁ : DMapLike γ₁ α β] [inst₂ : DMapLike γ₂ α β]
+  {m₁ : γ₁} {m₂ : γ₂} : keyEquiv (β:=β) m₁ m₂ ↔ keySubset (β:=β) m₁ m₂ ∧ keySubset (β:=β) m₂ m₁ := by
+  simp only [keySubset, keyEquiv]; apply Iff.intro <;> intro h
+  case mp => simp [h]
+  case mpr => intro x; apply Iff.intro <;> simp_all
+
+theorem DMapLike.equiv'_iff_subset {γ₁ γ₂ α β} [inst₁ : DMapLike γ₁ α β] [inst₂ : DMapLike γ₂ α β]
+  {m₁ : γ₁} {m₂ : γ₂} : equiv' (β:=β) m₁ m₂ ↔ subset (β:=β) m₁ m₂ ∧ subset (β:=β) m₂ m₁ := by
+  simp only [subset, equiv']; apply Iff.intro <;> intro h
+  case mp => simp [h]
+  case mpr =>
+    intro x
+    have h₁ := h.left x; have h₂ := h.right x
+    revert h₁ h₂ <;> cases m₁[x]ᵈ? <;> cases m₂[x]ᵈ? <;> simp
+
+open DMapLike
+
+/--
+  A finite dependently typed map where the behavior of
+  `· ∈ m , m[·]?, m[·]!, m[·], emptyWithCapacity, insert, erase, size`
+  are uniquely determined up to `Map.equiv`
+-/
+class LawfulDMapLike (γ : Type u) (α : Type v) (β : α → Type w) [inst : DMapLike γ α β]
+  extends LawfulMemSize γ α, LawfulDGetElem γ α β (fun m x => x ∈ m) where
+  not_mem_empty : ∀ {k : α} {n : Nat}, ¬ k ∈ emptyWithCapacity (self:=inst) n
+  mem_iff_isSome_dGetElem? : ∀ {m : γ} {k : α}, k ∈ m ↔ m[k]ᵈ?.isSome
+  dGetElem?_insert_self : ∀ {m : γ} {k : α} {v : β k}, (insert m k v)[k]ᵈ? = .some v
+  dGetElem?_insert_ne : ∀ {m : γ} {k a : α} {v : β k}, k ≠ a → (insert m k v)[a]ᵈ? = m[a]ᵈ?
+  dGetElem?_erase_self : ∀ {m : γ} {k : α}, (erase (β:=β) m k)[k]ᵈ? = .none
+  dGetElem?_erase_ne : ∀ {m : γ} {k a : α}, k ≠ a → (erase (β:=β) m k)[a]ᵈ? = m[a]ᵈ?
+  size_erase_mem : ∀ {m : γ} {k : α}, k ∈ m → Size.size (erase (β:=β) m k) + 1 = Size.size m
+
+theorem LawfulDMapLike.mem_iff_dGetElem?_eq_some {γ α β} [inst : DMapLike γ α β] [LawfulDMapLike γ α β] {m : γ} {k : α} : k ∈ m ↔ ∃ v, m[k]ᵈ? = .some v := by
+  rw [mem_iff_isSome_dGetElem?]; rw [Option.isSome_iff_exists]
+
+theorem LawfulDMapLike.not_mem_iff_dGetElem?_eq_none {γ α β} [inst : DMapLike γ α β] [LawfulDMapLike γ α β] {m : γ} {k : α} : k ∉ m ↔ m[k]ᵈ? = .none := by
+  rw [mem_iff_isSome_dGetElem?]; simp
+
+theorem LawfulDMapLike.mem_insert {γ α β} [inst : DMapLike γ α β] [LawfulDMapLike γ α β] {m : γ} {k a : α} {v : β k} :
+  a ∈ insert m k v ↔ (k = a) ∨ a ∈ m := by
+  rw [mem_iff_isSome_dGetElem?]; by_cases k = a
+  case pos h => cases h; simp [dGetElem?_insert_self]
+  case neg h => simp only [dGetElem?_insert_ne h]; simp [← mem_iff_isSome_dGetElem?, *]
+
+theorem LawfulDMapLike.mem_erase {γ α β} [inst : DMapLike γ α β] [LawfulDMapLike γ α β] {m : γ} {k a : α} :
+  a ∈ erase (β:=β) m k ↔ k ≠ a ∧ a ∈ m := by
+  rw [mem_iff_isSome_dGetElem?]; by_cases k = a
+  case pos h => cases h; simp [dGetElem?_erase_self]
+  case neg h => simp only [dGetElem?_erase_ne h]; simp [← mem_iff_isSome_dGetElem?, h]
+
+open Classical in
+theorem LawfulDMapLike.dGetElem?_eq_none_iff {γ α β} [inst : DMapLike γ α β] [LawfulDMapLike γ α β]
+  {c : γ} {i : α} : c[i]ᵈ? = .none ↔ i ∉ c := by
+  simp only [dGetElem?_def]
+  split <;> simp_all
+
+open Classical in
+theorem LawfulDMapLike.dGetElem?_eq_some_dGetElem {γ α β} [inst : DMapLike γ α β] [LawfulDMapLike γ α β] {m : γ} {k : α} (h : k ∈ m) :
+  m[k]ᵈ? = .some (m[k]ᵈ'h) := by
+  simp [dGetElem?_def, h]
+
+theorem LawfulDMapLike.dGetElem!_eq_dGetElem {γ α β} [inst : DMapLike γ α β] [LawfulDMapLike γ α β] {m : γ} {k : α} [Inhabited (β k)] (h : k ∈ m) :
+  m[k]ᵈ! = m[k]ᵈ'h := by
+  simp [dGetElem!_def, dGetElem?_eq_some_dGetElem h]
+
+theorem LawfulDMapLike.dGetElem!_eq_default {γ α β} [inst : DMapLike γ α β] [LawfulDMapLike γ α β] {m : γ} {k : α} [Inhabited (β k)] (h : k ∉ m) :
+  m[k]ᵈ! = default := by
+  simp [dGetElem!_def, dGetElem?_eq_none_iff.mpr h]
+
+theorem LawfulDMapLike.dGetElem!_eq_get!_dGetElem? {γ α β} [inst : DMapLike γ α β] [LawfulDMapLike γ α β] {m : γ} {k : α} [Inhabited (β k)] : m[k]ᵈ! = m[k]ᵈ?.get! := by
+  simp only [dGetElem!_def]; split <;> simp [*]
+
+theorem LawfulDMapLike.dGetElem?_eq_some_dGetElem! {γ α β} [inst : DMapLike γ α β] [LawfulDMapLike γ α β] {m : γ} {k : α} [Inhabited (β k)] (h : k ∈ m) :
+  m[k]ᵈ? = .some m[k]ᵈ! := by
+  simp [dGetElem?_eq_some_dGetElem h, dGetElem!_eq_dGetElem h]
+
+theorem LawfulDMapLike.dGetElem?_eq_none {γ α β} [inst : DMapLike γ α β] [LawfulDMapLike γ α β] {m : γ} {k : α} [Inhabited (β k)] (h : k ∉ m) :
+  m[k]ᵈ? = .none := by
+  simp [dGetElem?_eq_none_iff.mpr h]
+
+theorem LawfulDMapLike.dGetElem_eq_iff_dGetElem?_eq_some {γ α β} [inst : DMapLike γ α β] [LawfulDMapLike γ α β] {m : γ} {k : α} {v : β k} (h : k ∈ m) :
+  m[k]ᵈ'h = v ↔ m[k]ᵈ? = .some v := by
+  rw [dGetElem?_eq_some_dGetElem h]; simp
+
+theorem LawfulDMapLike.dGetElem_eq_of_dGetElem?_eq_some {γ α β} [inst : DMapLike γ α β] [LawfulDMapLike γ α β] {m : γ} {k : α} {v : β k}
+  (h : m[k]ᵈ? = .some v) : m[k]ᵈ'(mem_iff_dGetElem?_eq_some.mpr ⟨_, h⟩) = v := by
+  apply (LawfulDMapLike.dGetElem_eq_iff_dGetElem?_eq_some _).mpr h
+
+theorem LawfulDMapLike.dGetElem_eq_dGetElem_iff_dGetElem?_eq_dGetElem? {γ α β} [inst : DMapLike γ α β] [LawfulDMapLike γ α β] {m₁ m₂ : γ} {k : α}
+  (h₁ : k ∈ m₁) (h₂ : k ∈ m₂) : m₁[k]ᵈ'h₁ = m₂[k]ᵈ'h₂ ↔ m₁[k]ᵈ? = m₂[k]ᵈ? := by
+  rw [dGetElem?_eq_some_dGetElem h₁, dGetElem?_eq_some_dGetElem h₂]; simp
+
+theorem LawfulDMapLike.dGetElem_insert_self {γ α β} [inst : DMapLike γ α β] [LawfulDMapLike γ α β] {m : γ} {k : α} {v : β k} :
+  (insert m k v)[k]ᵈ'(mem_insert.mpr (Or.inl rfl)) = v := by
+  have hmem : k ∈ insert m k v := mem_insert.mpr (Or.inl rfl)
+  have heq := dGetElem?_eq_some_dGetElem hmem
+  rw [dGetElem?_insert_self] at heq
+  injection heq with heq; rw [← heq]
+
+theorem LawfulDMapLike.dGetElem_insert_ne {γ α β} [inst : DMapLike γ α β] [LawfulDMapLike γ α β] {m : γ} {k a : α} {v : β k} (h₁ : a ∈ insert m k v) (h₂ : k ≠ a) :
+  (insert m k v)[a]ᵈ'h₁ = m[a]ᵈ'(Or.resolve_left (mem_insert.mp h₁) h₂) := by
+  have heq := dGetElem?_eq_some_dGetElem h₁
+  have heq' := dGetElem?_eq_some_dGetElem (Or.resolve_left (mem_insert.mp h₁) h₂)
+  rw [dGetElem?_insert_ne h₂, heq'] at heq
+  injection heq with heq; rw [← heq]
+
+theorem LawfulDMapLike.dGetElem_erase {γ α β} [inst : DMapLike γ α β] [LawfulDMapLike γ α β] {m : γ} {k a : α} (h' : a ∈ erase m k) :
+  (erase (β:=β) m k)[a]ᵈ'h' = m[a]ᵈ'((mem_erase.mp h').right) := by
+  have heq := dGetElem?_eq_some_dGetElem h'
+  have heq' := dGetElem?_eq_some_dGetElem (mem_erase.mp h').right
+  by_cases k = a
+  case pos h => cases h; simp [dGetElem?_erase_self] at heq
+  case neg h =>
+    simp only [dGetElem?_erase_ne h, heq'] at heq
+    injection heq with heq; rw [← heq]
+
+theorem LawfulDMapLike.insert_mem_keyEquiv {γ α β} [inst : DMapLike γ α β] [LawfulDMapLike γ α β]
+  {m : γ} {k : α} {v : β k} (hmem : k ∈ m) : keyEquiv (β:=β) (insert m k v) m := by
+  simp [keyEquiv, mem_insert, hmem]
+
+theorem LawfulDMapLike.erase_insert_not_mem_equiv {γ α β} [inst : DMapLike γ α β] [LawfulDMapLike γ α β]
+  {m : γ} {k : α} {v : β k} (hnmem : k ∉ m) : equiv (β:=β) (erase (β:=β) (insert m k v) k) m := by
+  simp only [equiv, keyEquiv, mem_erase, mem_insert, dGetElem_erase]
+  apply And.intro
+  case left => intro x; by_cases (k = x) <;> simp_all
+  case right => intro x ⟨hne, h₁⟩ h₂; simp [dGetElem_insert_ne _ hne]
+
+theorem LawfulDMapLike.erase_not_mem_equiv {γ α β} [inst : DMapLike γ α β] [LawfulDMapLike γ α β]
+  {m : γ} {k : α} (hnmem : k ∉ m) : equiv (β:=β) (erase (β:=β) m k) m := by
+  simp only [equiv, keyEquiv, mem_erase, dGetElem_erase]
+  apply And.intro
+  case left => intro x; by_cases (k = x) <;> simp_all
+  case right => simp
+
+theorem LawfulDMapLike.insert_erase_mem_keyEquiv {γ α β} [inst : DMapLike γ α β] [LawfulDMapLike γ α β]
+  {m : γ} {k : α} {v : β k} (hmem : k ∈ m) : keyEquiv (β:=β) (insert (erase (β:=β) m k) k v) m := by
+  simp only [keyEquiv, mem_insert, mem_erase]
+  intro x; by_cases (k = x) <;> simp_all
+
+theorem LawfulDMapLike.insert_erase_dGetElem_eq_equiv {γ α β} [inst : DMapLike γ α β] [LawfulDMapLike γ α β]
+  {m : γ} {k : α} {v : β k} (hmem : k ∈ m) (hget : m[k]ᵈ'hmem = v) : equiv (β:=β) (insert (erase (β:=β) m k) k v) m := by
+  simp only [equiv, keyEquiv, mem_insert, mem_erase]
+  apply And.intro
+  case left => intro x; grind
+  case right =>
+    intro x h₁ h₂; cases h₁
+    case inl heq => cases heq; simp [dGetElem_insert_self, hget]
+    case inr hne => simp [dGetElem_insert_ne _ hne.left, dGetElem_erase]
+
+theorem LawfulDMapLike.exists_key_list {γ α β} [inst : DMapLike γ α β] [LawfulDMapLike γ α β] {m : γ} :
+  ∃ (l : List α), l.length = Size.size m ∧ l.Nodup ∧ ∀ k, k ∈ m ↔ k ∈ l := by
+  generalize hsz : Size.size m = n
+  induction n generalizing m
+  case zero =>
+    exists []; simp [LawfulMemSize.size_zero_iff_forall_not_mem.mp hsz]
+  case succ n IH =>
+    have hnz : Size.size m ≠ 0 := by
+      intro h; rw [h] at hsz; simp at hsz
+    have ⟨x, hx⟩ := LawfulMemSize.size_ne_zero_iff_exists_mem.mp hnz
+    let me := erase (β:=β) m x
+    have hmesz : Size.size (erase (β:=β) m x) = n := by
+      have := (size_erase_mem hx).trans hsz; simp_all
+    have ⟨l, hlen, hnd, hequiv⟩ := IH hmesz
+    exists x::l
+    apply And.intro ?len (And.intro ?nd ?equiv)
+    case len => simp [hlen]
+    case nd => simp [← hequiv, hnd, mem_erase]
+    case equiv =>
+      simp only [List.mem_cons, ← hequiv, mem_erase]
+      intro k; apply Iff.intro
+      case mp => intro hk; grind
+      case mpr => intro hk; cases hk <;> simp [*]
+
+noncomputable def LawfulDMapLike.exKeyList {γ α β} [inst : DMapLike γ α β] [LawfulDMapLike γ α β] (m : γ) : List α :=
+  (exists_key_list (α:=α) (β:=β) (m:=m)).choose
+
+noncomputable def LawfulDMapLike.length_exKeyList_eq_size {γ α β} [inst : DMapLike γ α β] [LawfulDMapLike γ α β] {m : γ} :
+  (exKeyList (α:=α) (β:=β) m).length = Size.size m :=
+  (Exists.choose_spec exists_key_list).left
+
+noncomputable def LawfulDMapLike.length_exKeyList_nodup {γ α β} [inst : DMapLike γ α β] [LawfulDMapLike γ α β] {m : γ} :
+  (exKeyList (α:=α) (β:=β) m).Nodup :=
+  (Exists.choose_spec exists_key_list).right.left
+
+noncomputable def LawfulDMapLike.length_exKeyList_equiv {γ α β} [inst : DMapLike γ α β] [LawfulDMapLike γ α β] {m : γ} :
+  ∀ k, k ∈ m ↔ k ∈ (exKeyList (α:=α) (β:=β) m) :=
+  (Exists.choose_spec exists_key_list).right.right
+
+theorem LawfulDMapLike.size_le_of_keySubset {γ₁ γ₂ α β} [inst₁ : DMapLike γ₁ α β] [inst₂ : DMapLike γ₂ α β]
+  [LawfulDMapLike γ₁ α β] [LawfulDMapLike γ₂ α β] {m₁ : γ₁} {m₂ : γ₂}
+  (hsub : keySubset (β:=β) m₁ m₂) : Size.size m₁ ≤ Size.size m₂ := by
+  let ⟨l₁, heq₁, hnd₁, hequiv₁⟩ := exists_key_list (inst:=inst₁) (m:=m₁)
+  let ⟨l₂, heq₂, hnd₂, hequiv₂⟩ := exists_key_list (inst:=inst₂) (m:=m₂)
+  rw [← heq₁, ← heq₂]
+  apply List.length_le_of_subset hnd₁
+  intro x hx
+  rw [← hequiv₂]; apply hsub; rw [hequiv₁]; exact hx
+
+theorem LawfulDMapLike.size_eq_of_keyEquiv {γ₁ γ₂ α β} [inst₁ : DMapLike γ₁ α β] [inst₂ : DMapLike γ₂ α β]
+  [LawfulDMapLike γ₁ α β] [LawfulDMapLike γ₂ α β] {m₁ : γ₁} {m₂ : γ₂}
+  (hequiv : keyEquiv (β:=β) m₁ m₂) : Size.size m₁ = Size.size m₂ := by
+  rw [keyEquiv_iff_keySubset] at hequiv
+  have h₁ := size_le_of_keySubset hequiv.left
+  have h₂ := size_le_of_keySubset hequiv.right
+  omega
+
+theorem LawfulDMapLike.keyEquiv_iff_size_eq_and_keySubset {γ₁ γ₂ α β} [inst₁ : DMapLike γ₁ α β] [inst₂ : DMapLike γ₂ α β]
+  [LawfulDMapLike γ₁ α β] [LawfulDMapLike γ₂ α β] {m₁ : γ₁} {m₂ : γ₂} :
+  keyEquiv (β:=β) m₁ m₂ ↔ Size.size m₁ = Size.size m₂ ∧ keySubset (β:=β) m₁ m₂ := by
+  let ⟨l₁, heq₁, hnd₁, hequiv₁⟩ := exists_key_list (β:=β) (m:=m₁)
+  let ⟨l₂, heq₂, hnd₂, hequiv₂⟩ := exists_key_list (β:=β) (m:=m₂)
+  simp only [keyEquiv, keySubset]
+  rw [← heq₁, ← heq₂]; simp only [hequiv₁, hequiv₂]
+  simp only [← List.nodup_perm_iff_equiv hnd₁ hnd₂,
+             ← List.subset_def,
+             ← List.nodup_subPerm_iff_subset hnd₁ hnd₂]
+  apply List.perm_iff_length_eq_andsubPerm
+
+theorem LawfulDMapLike.size_insert_mem {γ α β} [inst : DMapLike γ α β] [LawfulDMapLike γ α β] {m : γ}
+  {k : α} {v : β k} (hmem : k ∈ m) : Size.size (insert m k v) = Size.size m := by
+  apply size_eq_of_keyEquiv; apply insert_mem_keyEquiv hmem
+
+theorem LawfulDMapLike.size_insert_not_mem {γ α β} [inst : DMapLike γ α β] [LawfulDMapLike γ α β] {m : γ}
+  {k : α} {v : β k} (hnmem : k ∉ m) : Size.size (insert m k v) = Size.size m + 1 := by
+  have hke := erase_insert_not_mem_equiv hnmem (v:=v)
+  rw [← size_eq_of_keyEquiv hke.left]; symm
+  apply size_erase_mem; simp [mem_insert]
+
+theorem LawfulDMapLike.size_insert_le {γ α β} [inst : DMapLike γ α β] [LawfulDMapLike γ α β] {m : γ}
+  {k : α} {v : β k} : Size.size (insert m k v) ≤ Size.size m + 1 := by
+  by_cases k ∈ m
+  case pos h => rw [size_insert_mem h]; simp
+  case neg h => rw [size_insert_not_mem h]; exact .refl
+
+theorem LawfulDMapLike.le_size_insert {γ α β} [inst : DMapLike γ α β] [LawfulDMapLike γ α β] {m : γ}
+  {k : α} {v : β k} : Size.size m ≤ Size.size (insert m k v) := by
+  by_cases k ∈ m
+  case pos h => rw [size_insert_mem h]; exact .refl
+  case neg h => rw [size_insert_not_mem h]; simp
+
+theorem LawfulDMapLike.size_insert_gt_zero {γ α β} [inst : DMapLike γ α β] [LawfulDMapLike γ α β] {m : γ}
+  {k : α} {v : β k} : Size.size (insert m k v) > 0 := by
+  by_cases k ∈ m
+  case pos h => rw [size_insert_mem h]; apply LawfulMemSize.size_gt_zero_iff_exists_mem.mpr ⟨_, h⟩
+  case neg h => rw [size_insert_not_mem h]; simp
+
+theorem LawfulDMapLike.size_erase_not_mem {γ α β} [inst : DMapLike γ α β] [LawfulDMapLike γ α β] {m : γ}
+  {k : α} (hnm : k ∉ m) : Size.size (erase (β:=β) m k) = Size.size m := by
+  apply size_eq_of_keyEquiv; apply (erase_not_mem_equiv hnm).left
+
+theorem LawfulDMapLike.size_erase_le {γ α β} [inst : DMapLike γ α β] [LawfulDMapLike γ α β] {m : γ}
+  {k : α} : Size.size (erase (β:=β) m k) ≤ Size.size m := by
+  by_cases k ∈ m
+  case pos h => have := size_erase_mem h; omega
+  case neg h => rw [size_erase_not_mem h]; exact .refl
+
+theorem LawfulDMapLike.le_size_erase {γ α β} [inst : DMapLike γ α β] [LawfulDMapLike γ α β] {m : γ}
+  {k : α} : Size.size m ≤ Size.size (erase (β:=β) m k) + 1 := by
+  by_cases k ∈ m
+  case pos h => simp [size_erase_mem h]
+  case neg h => rw [size_erase_not_mem h]; simp
+
+theorem LawfulDMapLike.dGetElem?_empty {γ α β} [inst : DMapLike γ α β] [LawfulDMapLike γ α β]
+  {capacity : Nat} {k : α} : (emptyWithCapacity (γ:=γ) (β:=β) capacity)[k]ᵈ? = .none := by
+  rw [← not_mem_iff_dGetElem?_eq_none]; apply not_mem_empty
+
+theorem LawfulDMapLike.dGetElem?_insert {γ α β} [inst : DMapLike γ α β]
+  [LawfulDMapLike γ α β] [DecidableEq α] {m : γ} {k a : α} {v : β k} :
+  (insert m k v)[a]ᵈ? = if h : k = a then h ▸ some v else m[a]ᵈ? := by
+  by_cases (a ∈ insert m k v)
+  case pos h =>
+    rw [mem_insert] at h; by_cases (k = a)
+    case pos heq => cases heq; simp [dGetElem?_insert_self]
+    case neg heq => simp [dGetElem?_insert_ne heq, heq]
+  case neg h =>
+    rw [not_mem_iff_dGetElem?_eq_none.mp h]
+    rw [mem_insert, not_or] at h
+    simp [not_mem_iff_dGetElem?_eq_none.mp h.right, h.left]
+
+theorem LawfulDMapLike.dGetElem?_erase {γ α β} [inst : DMapLike γ α β]
+  [LawfulDMapLike γ α β] [DecidableEq α] {m : γ} {k a : α} :
+  (erase (β:=β) m k)[a]ᵈ? = if (k = a) then .none else m[a]ᵈ? := by
+  by_cases k = a
+  case pos h => cases h; simp [dGetElem?_erase_self]
+  case neg h => simp [dGetElem?_erase_ne h, h]
+
+open Classical in
+theorem LawfulDMapLike.dGetElem?_eq_none_iff_dGetElem?_eq_none_of_keyEquiv {γ₁ γ₂ α β}
+  [inst₁ : DMapLike γ₁ α β] [inst₂ : DMapLike γ₂ α β] [LawfulDMapLike γ₁ α β] [LawfulDMapLike γ₂ α β]
+  {m₁ : γ₁} {m₂ : γ₂} (hequiv : DMapLike.keyEquiv (β:=β) m₁ m₂)
+  (k : α) : m₁[k]ᵈ? = .none ↔ m₂[k]ᵈ? = .none := by
+  simp [dGetElem?_eq_none_iff, hequiv k]
+
+theorem LawfulDMapLike.equiv_iff_equiv' {γ₁ γ₂ α β}
+  [inst₁ : DMapLike γ₁ α β] [inst₂ : DMapLike γ₂ α β] [LawfulDMapLike γ₁ α β] [LawfulDMapLike γ₂ α β]
+  {m₁ : γ₁} {m₂ : γ₂} :
+  DMapLike.equiv (β:=β) m₁ m₂ ↔ DMapLike.equiv' (β:=β) m₁ m₂ := by
+  simp only [equiv, equiv']; apply Iff.intro
+  case mp =>
+    intro ⟨hk, hv⟩ x
+    cases h₁ : m₁[x]ᵈ?
+    case none =>
+      simp [(dGetElem?_eq_none_iff_dGetElem?_eq_none_of_keyEquiv hk _).mp h₁]
+    case some =>
+      have hxm₁ := @mem_iff_dGetElem?_eq_some.mpr ⟨_, h₁⟩
+      rw [dGetElem?_eq_some_dGetElem hxm₁,
+          hv _ hxm₁ ((hk _).mp hxm₁), ← dGetElem?_eq_some_dGetElem] at h₁
+      simp [h₁]
+  case mpr =>
+    intro h?; apply And.intro
+    case left => intro x; simp [mem_iff_dGetElem?_eq_some, h?]
+    case right =>
+      intro x h₁ h₂
+      apply Option.some.inj
+      simp only [← dGetElem?_eq_some_dGetElem, h?]
+
+theorem LawfulDMapLike.equiv_iff_subset {γ₁ γ₂ α β}
+  [inst₁ : DMapLike γ₁ α β] [inst₂ : DMapLike γ₂ α β] [LawfulDMapLike γ₁ α β] [LawfulDMapLike γ₂ α β]
+  {m₁ : γ₁} {m₂ : γ₂} : equiv (β:=β) m₁ m₂ ↔ subset (β:=β) m₁ m₂ ∧ subset (β:=β) m₂ m₁ := by
+  rw [LawfulDMapLike.equiv_iff_equiv', DMapLike.equiv'_iff_subset]
+
+theorem LawfulDMapLike.keySubset_of_subset {γ₁ γ₂ α β}
+  [inst₁ : DMapLike γ₁ α β] [inst₂ : DMapLike γ₂ α β] [LawfulDMapLike γ₁ α β] [LawfulDMapLike γ₂ α β]
+  {m₁ : γ₁} {m₂ : γ₂} (h : subset (β:=β) m₁ m₂) : keySubset (β:=β) m₁ m₂ := by
+  simp only [subset] at h
+  intro x
+  simp only [mem_iff_isSome_dGetElem?]
+  have hx := h x
+  revert hx
+  cases m₁[x]ᵈ? <;> grind
+
+theorem LawfulDMapLike.mem_congr {γ₁ γ₂ α β} [inst₁ : DMapLike γ₁ α β] [inst₂ : DMapLike γ₂ α β]
+  [LawfulDMapLike γ₁ α β] [LawfulDMapLike γ₂ α β] {m₁ : γ₁} {m₂ : γ₂}
+  (hequiv : equiv (β:=β) m₁ m₂) (x : α) : x ∈ m₁ ↔ x ∈ m₂ := hequiv.left _
+
+theorem LawfulDMapLike.dGetElem?_congr {γ₁ γ₂ α β} [inst₁ : DMapLike γ₁ α β] [inst₂ : DMapLike γ₂ α β]
+  [LawfulDMapLike γ₁ α β] [LawfulDMapLike γ₂ α β] {m₁ : γ₁} {m₂ : γ₂}
+  (hequiv : equiv (β:=β) m₁ m₂) (x : α) : m₁[x]ᵈ? = m₂[x]ᵈ? :=
+  LawfulDMapLike.equiv_iff_equiv'.mp hequiv _
+
+theorem LawfulDMapLike.dGetElem_congr {γ₁ γ₂ α β} [inst₁ : DMapLike γ₁ α β] [inst₂ : DMapLike γ₂ α β]
+  [LawfulDMapLike γ₁ α β] [LawfulDMapLike γ₂ α β] {m₁ : γ₁} {m₂ : γ₂}
+  (hequiv : equiv (β:=β) m₁ m₂) (x : α) (h₁ : x ∈ m₁) (h₂ : x ∈ m₂) : m₁[x]ᵈ'h₁ = m₂[x]ᵈ'h₂ := by
+  have heq := LawfulDMapLike.dGetElem?_congr hequiv x
+  simp only [dGetElem?_eq_some_dGetElem h₁,
+             dGetElem?_eq_some_dGetElem h₂] at heq
+  injection heq
+
+theorem LawfulDMapLike.dGetElem_congr' {γ₁ γ₂ α β} [inst₁ : DMapLike γ₁ α β] [inst₂ : DMapLike γ₂ α β]
+  [LawfulDMapLike γ₁ α β] [LawfulDMapLike γ₂ α β] {m₁ : γ₁} {m₂ : γ₂}
+  (hequiv : equiv (β:=β) m₁ m₂) (x : α) (h₁ : x ∈ m₁) : m₁[x]ᵈ'h₁ = m₂[x]ᵈ'((hequiv.left _).mp h₁) := by
+  have heq := LawfulDMapLike.dGetElem?_congr hequiv x
+  simp only [dGetElem?_eq_some_dGetElem h₁,
+             dGetElem?_eq_some_dGetElem ((hequiv.left _).mp h₁)] at heq
+  injection heq
+
+theorem LawfulDMapLike.dGetElem!_congr {γ₁ γ₂ α β} [inst₁ : DMapLike γ₁ α β] [inst₂ : DMapLike γ₂ α β]
+  [LawfulDMapLike γ₁ α β] [LawfulDMapLike γ₂ α β] {m₁ : γ₁} {m₂ : γ₂}
+  (hequiv : equiv (β:=β) m₁ m₂) (x : α) [Inhabited (β x)] : m₁[x]ᵈ! = m₂[x]ᵈ! := by
+  simp [dGetElem!_def, LawfulDMapLike.dGetElem?_congr hequiv]
+
+theorem LawfulDMapLike.emptyWithCapacity_congr {γ₁ γ₂ α β} [inst₁ : DMapLike γ₁ α β] [inst₂ : DMapLike γ₂ α β]
+  [LawfulDMapLike γ₁ α β] [LawfulDMapLike γ₂ α β] (capacity₁ capacity₂ : Nat) :
+  equiv (β:=β) (inst₂:=inst₂)
+    (emptyWithCapacity (self:=inst₁) capacity₁)
+    (emptyWithCapacity (self:=inst₂) capacity₂) := by
+  rw [equiv_iff_equiv']; intro x
+  simp [dGetElem?_empty]
+
+open Classical in
+theorem LawfulDMapLike.insert_congr {γ₁ γ₂ α β} [inst₁ : DMapLike γ₁ α β] [inst₂ : DMapLike γ₂ α β]
+  [LawfulDMapLike γ₁ α β] [LawfulDMapLike γ₂ α β] {m₁ : γ₁} {m₂ : γ₂}
+  (hequiv : equiv (β:=β) m₁ m₂) (k : α) (v : β k) :
+  equiv (β:=β) (insert m₁ k v) (insert m₂ k v) := by
+  rw [equiv_iff_equiv']
+  intro x
+  simp [dGetElem?_insert, equiv_iff_equiv'.mp hequiv _]
+
+open Classical in
+theorem LawfulDMapLike.erase_congr {γ₁ γ₂ α β} [inst₁ : DMapLike γ₁ α β] [inst₂ : DMapLike γ₂ α β]
+  [LawfulDMapLike γ₁ α β] [LawfulDMapLike γ₂ α β] {m₁ : γ₁} {m₂ : γ₂}
+  (hequiv : equiv (β:=β) m₁ m₂) (k : α) :
+  equiv (β:=β) (erase m₁ (self:=inst₁) k) (erase m₂ (self:=inst₂) k) := by
+  rw [equiv_iff_equiv']
+  intro x
+  simp [dGetElem?_erase, equiv_iff_equiv'.mp hequiv _]
+
+theorem LawfulDMapLike.size_congr {γ₁ γ₂ α β} [inst₁ : DMapLike γ₁ α β] [inst₂ : DMapLike γ₂ α β]
+  [LawfulDMapLike γ₁ α β] [LawfulDMapLike γ₂ α β] {m₁ : γ₁} {m₂ : γ₂}
+  (hequiv : equiv (β:=β) m₁ m₂) : Size.size m₁ = Size.size m₂ := by
+  apply LawfulDMapLike.size_eq_of_keyEquiv; exact hequiv.left
+
+instance {α β} [BEq α] [Hashable α] [LawfulBEq α] : DMapLike (DHashMap α β) α β where
+  emptyWithCapacity capacity := DHashMap.emptyWithCapacity (capacity:=capacity)
+  insert := DHashMap.insert
+  erase := DHashMap.erase
+  size := DHashMap.size
+
+instance {α β} [BEq α] [Hashable α] [LawfulBEq α] : LawfulDMapLike (DHashMap α β) α β where
+  not_mem_empty := by intro k n; simp [DMapLike.emptyWithCapacity]
+  mem_iff_isSome_dGetElem? := DHashMap.mem_iff_isSome_get?
+  dGetElem?_insert_self := DHashMap.get?_insert_self
+  dGetElem?_insert_ne := by
+    intro m k a v h
+    simp [DMapLike.insert, dGetElem?, DHashMap.get?_insert, h]
+  dGetElem?_erase_self := DHashMap.get?_erase_self
+  dGetElem?_erase_ne := by
+    intro m k a h
+    simp [DMapLike.erase, dGetElem?, DHashMap.get?_erase, h]
+  size_zero_iff_forall_not_mem := by
+    intro m; simp only [Size.size]
+    apply DHashMap.size_zero_iff_forall_not_mem
+  size_erase_mem := DHashMap.size_erase_mem
+
+instance {α β} [Ord α] [LawfulEqOrd α] : DMapLike (DTreeMap α β) α β where
+  emptyWithCapacity _ := DTreeMap.empty
+  insert := DTreeMap.insert
+  erase := DTreeMap.erase
+  size := DTreeMap.size
+
+instance {α β} [Ord α] [LawfulEqOrd α] [TransOrd α] : LawfulDMapLike (DTreeMap α β) α β where
+  not_mem_empty := DTreeMap.not_mem_emptyc
+  mem_iff_isSome_dGetElem? := DTreeMap.mem_iff_isSome_get?
+  dGetElem?_insert_self := DTreeMap.get?_insert_self
+  dGetElem?_insert_ne := by
+    intro m k a v hne
+    simp only [DMapLike.insert, dGetElem?, DTreeMap.get?_insert]
+    rw [dite_cond_eq_false]
+    rw [LawfulEqOrd.compare_eq_iff_eq]
+    simp [hne]
+  dGetElem?_erase_self := DTreeMap.get?_erase_self
+  dGetElem?_erase_ne := by
+    intro m k a hne
+    simp only [DMapLike.erase, dGetElem?, DTreeMap.get?_erase]
+    rw [ite_cond_eq_false]
+    rw [LawfulEqOrd.compare_eq_iff_eq]
+    simp [hne]
+  size_zero_iff_forall_not_mem := by
+    intro m
+    rw [← DTreeMap.isEmpty_iff_forall_not_mem,
+        DTreeMap.isEmpty_eq_size_eq_zero]
+    simp [Size.size]
+  size_erase_mem := DTreeMap.size_erase_mem
+
+instance {α β} [BEq α] [Hashable α] [LawfulBEq α] [LawfulHashable α] : DMapLike (ExtDHashMap α β) α β where
+  emptyWithCapacity capacity := ExtDHashMap.emptyWithCapacity capacity
+  insert := ExtDHashMap.insert
+  erase := ExtDHashMap.erase
+  size := ExtDHashMap.size
+
+instance {α β} [BEq α] [Hashable α] [LawfulBEq α] [LawfulHashable α] : LawfulDMapLike (ExtDHashMap α β) α β where
+  not_mem_empty := by
+    intro k n; simp [DMapLike.emptyWithCapacity]
+    apply ExtDHashMap.not_mem_empty
+  mem_iff_isSome_dGetElem? := ExtDHashMap.mem_iff_isSome_get?
+  dGetElem?_insert_self := ExtDHashMap.get?_insert_self
+  dGetElem?_insert_ne := by
+    intros m k a v hne
+    simp [DMapLike.insert, dGetElem?, ExtDHashMap.get?_insert, hne]
+  dGetElem?_erase_self := ExtDHashMap.get?_erase_self
+  dGetElem?_erase_ne := by
+    intros m k a hne
+    simp [DMapLike.erase, dGetElem?, ExtDHashMap.get?_erase, hne]
+  size_zero_iff_forall_not_mem := by
+    intro m
+    rw [← ExtDHashMap.eq_empty_iff_forall_not_mem,
+        ExtDHashMap.eq_empty_iff_size_eq_zero]
+    rfl
+  size_erase_mem := ExtDHashMap.size_erase_mem
+
+instance {α β} [Ord α] [LawfulEqOrd α] [TransOrd α] : DMapLike (ExtDTreeMap α β) α β where
+  emptyWithCapacity _ := ExtDTreeMap.empty
+  insert := ExtDTreeMap.insert
+  erase := ExtDTreeMap.erase
+  size := ExtDTreeMap.size
+
+instance {α β} [Ord α] [LawfulEqOrd α] [TransOrd α] : LawfulDMapLike (ExtDTreeMap α β) α β where
+  not_mem_empty := DTreeMap.not_mem_emptyc
+  mem_iff_isSome_dGetElem? := ExtDTreeMap.mem_iff_isSome_get?
+  dGetElem?_insert_self := ExtDTreeMap.get?_insert_self
+  dGetElem?_insert_ne := by
+    intro m k a v hne
+    simp only [DMapLike.insert, dGetElem?, ExtDTreeMap.get?_insert]
+    rw [dite_cond_eq_false]
+    rw [LawfulEqOrd.compare_eq_iff_eq]
+    simp [hne]
+  dGetElem?_erase_self := ExtDTreeMap.get?_erase_self
+  dGetElem?_erase_ne := by
+    intro m k a hne
+    simp only [DMapLike.erase, dGetElem?, ExtDTreeMap.get?_erase]
+    rw [ite_cond_eq_false]
+    rw [LawfulEqOrd.compare_eq_iff_eq]
+    simp [hne]
+  size_zero_iff_forall_not_mem := by
+    intro m
+    rw [← ExtDTreeMap.isEmpty_iff_forall_not_mem,
+        ExtDTreeMap.isEmpty_eq_size_eq_zero]
+    simp [Size.size]
+  size_erase_mem := ExtDTreeMap.size_erase_mem
+
+end DMapLike
+
+/-!
+  This section defines an abstract datatype `MapLike` and its lawful
+  counterpart `LawfulMapLike`. An instance `inst : MapLike γ α β` denotes
+  that `γ` models a finite map from `α` to `β`, i.e. a function
+  from a finite collection of elements of type `α` (i.e. the keys) to `β`.
+
+  `MapLike` is a subtype of `Membership` and `GetElem?`. Therefore,
+  `γ` must support `∈` and `[ ], [ ]?, [ ]!`. In addition, it
+  must support the following operations: `emptyWithCapacity`,
+  `insert`, `erase`, `size`
+  · `a ∈ m` iff `a` is present in the keys
+  · `emptyWithCapacity k` returns an empty map with capacity `k`.
+    The capacity parameter is present because of performance considerations.
+  · `insert m k v`: insert the key-value pair `(k, v)` to `m`. If
+    `k` is already present, its value is overriden
+  · `erase m k`: erase the key `k` from `m`
+  · `size m`: return the size of `m`
+
+  `LawfulMapLike` specifies the behavior of the operations supported by
+  `MapLike`, whereby the behavior of the operations are uniquely determined
+  up to `MapLike.equiv`.
+-/
+
+section MapLike
+
+/--
+  A finite map which supports insertion, deletion, lookup,
+  and computing size
+-/
+class MapLike (γ : Type u) (α : Type v) (β : Type w) extends
+  Membership α γ, GetElem? γ α β (fun m x => x ∈ m), Size γ where
+  emptyWithCapacity {γ α β} : Nat → γ
+  insert : γ → α → β → γ
+  erase {γ α β} : γ → α → γ
+
+def MapLike_of_DMapLike {γ α β} (inst : DMapLike γ α (fun _ => β)) : MapLike γ α β where
+  getElem := inst.dGetElem
+  getElem? := inst.dGetElem?
+  getElem! c i := inst.dGetElem! c i
+  emptyWithCapacity := inst.emptyWithCapacity
+  insert := inst.insert
+  erase := inst.erase
+  size := inst.size
+
+def DMapLike_of_MapLike {γ α β} (inst : MapLike γ α β) : DMapLike γ α (fun _ => β) where
+  dGetElem := inst.getElem
+  dGetElem? := inst.getElem?
+  dGetElem! c i := inst.getElem! c i
+  emptyWithCapacity := inst.emptyWithCapacity
+  insert := inst.insert
+  erase := inst.erase
+  size := inst.size
+
+def DMapLike_MapLike_inv {γ α β} {inst : DMapLike γ α (fun _ => β)} :
+  DMapLike_of_MapLike (MapLike_of_DMapLike inst) = inst := rfl
+
+def MapLike_DMapLike_inv {γ α β} {inst : MapLike γ α β} :
+  MapLike_of_DMapLike (DMapLike_of_MapLike inst) = inst := rfl
+
+def MapLike.keyEquiv {γ₁ γ₂ α β} [inst₁ : MapLike γ₁ α β] [inst₂ : MapLike γ₂ α β]
+  (m₁ : γ₁) (m₂ : γ₂) := ∀ (x : α), x ∈ m₁ ↔ x ∈ m₂
+
+def MapLike.equiv {γ₁ γ₂ α β} [inst₁ : MapLike γ₁ α β] [inst₂ : MapLike γ₂ α β] (m₁ : γ₁) (m₂ : γ₂) :=
+  keyEquiv (α:=α) (β:=β) m₁ m₂ ∧ ∀ (x : α) (h₁ : x ∈ m₁) (h₂ : x ∈ m₂), m₁[x] = m₂[x]
+
+def MapLike.equiv' {γ₁ γ₂ α β} [inst₁ : MapLike γ₁ α β] [inst₂ : MapLike γ₂ α β] (m₁ : γ₁) (m₂ : γ₂) :=
+  ∀ (x : α), m₁[x]? = m₂[x]?
+
+def MapLike.keySubset {γ₁ γ₂ α β} [inst₁ : MapLike γ₁ α β] [inst₂ : MapLike γ₂ α β] (m₁ : γ₁) (m₂ : γ₂) :=
+  ∀ (x : α), x ∈ m₁ → x ∈ m₂
+
+def MapLike.subset {γ₁ γ₂ α β} [inst₁ : MapLike γ₁ α β] [inst₂ : MapLike γ₂ α β] (m₁ : γ₁) (m₂ : γ₂) :=
+  ∀ (x : α) (y : β), m₁[x]? = y → m₂[x]? = y
+
+theorem MapLike.keyEquiv.refl {γ α β} [inst : MapLike γ α β] {m : γ} : keyEquiv (α:=α) (β:=β) m m := by
+  simp [keyEquiv]
+
+theorem MapLike.keyEquiv.comm {γ₁ γ₂ α β} [inst₁ : MapLike γ₁ α β] [inst₂ : MapLike γ₂ α β]
+  {m₁ : γ₁} {m₂ : γ₂} : keyEquiv (α:=α) (β:=β) m₁ m₂ ↔ keyEquiv (α:=α) (β:=β) m₂ m₁ :=
+  DMapLike.keyEquiv.comm (inst₁:=DMapLike_of_MapLike inst₁) (inst₂:=DMapLike_of_MapLike inst₂)
+
+theorem MapLike.keyEquiv.symm {γ₁ γ₂ α β} [inst₁ : MapLike γ₁ α β] [inst₂ : MapLike γ₂ α β]
+  {m₁ : γ₁} {m₂ : γ₂} : keyEquiv (α:=α) (β:=β) m₁ m₂ → keyEquiv (α:=α) (β:=β) m₂ m₁ :=
+  MapLike.keyEquiv.comm.mp
+
+theorem MapLike.keyEquiv.trans {γ₁ γ₂ γ₃ α β} [inst₁ : MapLike γ₁ α β] [inst₂ : MapLike γ₂ α β] [inst₃ : MapLike γ₃ α β]
+  {m₁ : γ₁} {m₂ : γ₂} {m₃ : γ₃} : keyEquiv (α:=α) (β:=β) m₁ m₂ → keyEquiv (α:=α) (β:=β) m₂ m₃ → keyEquiv (α:=α) (β:=β) m₁ m₃ := by
+  intro h₁ h₂ x
+  rw [h₁, h₂]
+
+theorem MapLike.equiv.refl {γ α β} [inst : MapLike γ α β] {m : γ} : equiv (α:=α) (β:=β) m m := by
+  simp [equiv, keyEquiv]
+
+theorem MapLike.equiv.comm {γ₁ γ₂ α β} [inst₁ : MapLike γ₁ α β] [inst₂ : MapLike γ₂ α β]
+  {m₁ : γ₁} {m₂ : γ₂} : equiv (α:=α) (β:=β) m₁ m₂ ↔ equiv (α:=α) (β:=β) m₂ m₁ :=
+  DMapLike.equiv.comm (inst₁:=DMapLike_of_MapLike inst₁) (inst₂:=DMapLike_of_MapLike inst₂)
+
+theorem MapLike.equiv.symm {γ₁ γ₂ α β} [inst₁ : MapLike γ₁ α β] [inst₂ : MapLike γ₂ α β]
+  {m₁ : γ₁} {m₂ : γ₂} : equiv (α:=α) (β:=β) m₁ m₂ → equiv (α:=α) (β:=β) m₂ m₁ :=
+  MapLike.equiv.comm.mp
+
+theorem MapLike.equiv.trans {γ₁ γ₂ γ₃ α β} [inst₁ : MapLike γ₁ α β] [inst₂ : MapLike γ₂ α β] [inst₃ : MapLike γ₃ α β]
+  {m₁ : γ₁} {m₂ : γ₂} {m₃ : γ₃} : equiv (α:=α) (β:=β) m₁ m₂ → equiv (α:=α) (β:=β) m₂ m₃ → equiv (α:=α) (β:=β) m₁ m₃ :=
+  DMapLike.equiv.trans (inst₁:=DMapLike_of_MapLike inst₁) (inst₂:=DMapLike_of_MapLike inst₂) (inst₃:=DMapLike_of_MapLike inst₃)
+
+theorem MapLike.equiv'.refl {γ α β} [inst : MapLike γ α β] {m : γ} : equiv' (α:=α) (β:=β) m m := by
+  simp [equiv']
+
+theorem MapLike.equiv'.comm {γ₁ γ₂ α β} [inst₁ : MapLike γ₁ α β] [inst₂ : MapLike γ₂ α β]
+  {m₁ : γ₁} {m₂ : γ₂} : equiv' (α:=α) (β:=β) m₁ m₂ ↔ equiv' (α:=α) (β:=β) m₂ m₁ :=
+  DMapLike.equiv'.comm (inst₁:=DMapLike_of_MapLike inst₁) (inst₂:=DMapLike_of_MapLike inst₂)
+
+theorem MapLike.equiv'.symm {γ₁ γ₂ α β} [inst₁ : MapLike γ₁ α β] [inst₂ : MapLike γ₂ α β]
+  {m₁ : γ₁} {m₂ : γ₂} : equiv' (α:=α) (β:=β) m₁ m₂ → equiv' (α:=α) (β:=β) m₂ m₁ :=
+  MapLike.equiv'.comm.mp
+
+theorem MapLike.equiv'.trans {γ₁ γ₂ γ₃ α β} [inst₁ : MapLike γ₁ α β] [inst₂ : MapLike γ₂ α β] [inst₃ : MapLike γ₃ α β]
+  {m₁ : γ₁} {m₂ : γ₂} {m₃ : γ₃} : equiv' (α:=α) (β:=β) m₁ m₂ → equiv' (α:=α) (β:=β) m₂ m₃ → equiv' (α:=α) (β:=β) m₁ m₃ := by
+  intro h₁ h₂ x; rw [h₁, h₂]
+
+theorem MapLike.keyEquiv_iff_keySubset {γ₁ γ₂ α β} [inst₁ : MapLike γ₁ α β] [inst₂ : MapLike γ₂ α β]
+  {m₁ : γ₁} {m₂ : γ₂} : keyEquiv (α:=α) (β:=β) m₁ m₂ ↔ keySubset (α:=α) (β:=β) m₁ m₂ ∧ keySubset (α:=α) (β:=β) m₂ m₁ := by
+  simp only [keySubset, keyEquiv]; apply Iff.intro <;> intro h
+  case mp => simp [h]
+  case mpr => intro x; apply Iff.intro <;> simp_all
+
+theorem MapLike.equiv'_iff_subset {γ₁ γ₂ α β} [inst₁ : MapLike γ₁ α β] [inst₂ : MapLike γ₂ α β]
+  {m₁ : γ₁} {m₂ : γ₂} : equiv' (α:=α) (β:=β) m₁ m₂ ↔ subset (α:=α) (β:=β) m₁ m₂ ∧ subset (α:=α) (β:=β) m₂ m₁ := by
+  simp only [subset, equiv']; apply Iff.intro <;> intro h
+  case mp => simp [h]
+  case mpr =>
+    intro x
+    have h₁ := h.left x; have h₂ := h.right x
+    revert h₁ h₂ <;> cases m₁[x]? <;> cases m₂[x]? <;> simp
+
+open MapLike
+
+/--
+  A finite map where the behavior of
+  `· ∈ m , m[·]?, m[·]!, m[·], emptyWithCapacity, insert, erase, size`
+  are uniquely determined up to `MapLike.equiv`
+-/
+class LawfulMapLike (γ : Type u) (α : Type v) (β : Type w) [inst : MapLike γ α β]
+  extends LawfulGetElem γ α β (fun m x => x ∈ m), LawfulMemSize γ α where
+  not_mem_empty : ∀ {k : α} {n : Nat}, ¬ k ∈ emptyWithCapacity (self:=inst) n
+  mem_iff_isSome_getElem? : ∀ {m : γ} {k : α}, k ∈ m ↔ m[k]?.isSome
+  getElem?_insert_self : ∀ {m : γ} {k : α} {v : β}, (insert m k v)[k]? = .some v
+  getElem?_insert_ne : ∀ {m : γ} {k a : α} {v : β}, k ≠ a → (insert m k v)[a]? = m[a]?
+  getElem?_erase_self : ∀ {m : γ} {k : α}, (erase (β:=β) m k)[k]? = .none
+  getElem?_erase_ne : ∀ {m : γ} {k a : α}, k ≠ a → (erase (β:=β) m k)[a]? = m[a]?
+  size_erase_mem : ∀ {m : γ} {k : α}, k ∈ m → Size.size (erase (β:=β) m k) + 1 = Size.size m
+
+def LawfulMapLike_of_LawfulDMapLike {γ α β} [inst : MapLike γ α β]
+  [instL : LawfulDMapLike (inst:=DMapLike_of_MapLike inst) γ α (fun _ => β)] :
+  LawfulMapLike γ α β where
+  getElem?_def := instL.dGetElem?_def
+  getElem!_def c i := by
+    have h := instL.dGetElem!_def c i
+    simp only [dGetElem!, dGetElem?, DMapLike_of_MapLike] at h
+    split at h <;> simp [*]
+  not_mem_empty := instL.not_mem_empty
+  mem_iff_isSome_getElem? := instL.mem_iff_isSome_dGetElem?
+  getElem?_insert_self := instL.dGetElem?_insert_self
+  getElem?_insert_ne := instL.dGetElem?_insert_ne
+  getElem?_erase_self := instL.dGetElem?_erase_self
+  getElem?_erase_ne := instL.dGetElem?_erase_ne
+  size_zero_iff_forall_not_mem := instL.size_zero_iff_forall_not_mem
+  size_erase_mem := instL.size_erase_mem
+
+theorem LawfulMapLike_of_LawfulDMapLike' {γ α β} [inst : DMapLike γ α (fun _ => β)]
+  [instL : LawfulDMapLike γ α (fun _ => β)] :
+  LawfulMapLike (inst:=MapLike_of_DMapLike inst) γ α β :=
+  LawfulMapLike_of_LawfulDMapLike (inst:=MapLike_of_DMapLike inst)
+
+def LawfulDMapLike_of_LawfulMapLike {γ α β} [inst : DMapLike γ α (fun _ => β)]
+  [instL : LawfulMapLike (inst:=MapLike_of_DMapLike inst) γ α β] :
+  LawfulDMapLike γ α (fun _ => β) where
+  dGetElem?_def := instL.getElem?_def
+  dGetElem!_def c i := by
+    intro _; have h := instL.getElem!_def c i
+    simp only [getElem!, getElem?, MapLike_of_DMapLike] at h
+    split at h <;> simp [*]
+  not_mem_empty := instL.not_mem_empty
+  mem_iff_isSome_dGetElem? := instL.mem_iff_isSome_getElem?
+  dGetElem?_insert_self := instL.getElem?_insert_self
+  dGetElem?_insert_ne := instL.getElem?_insert_ne
+  dGetElem?_erase_self := instL.getElem?_erase_self
+  dGetElem?_erase_ne := instL.getElem?_erase_ne
+  size_zero_iff_forall_not_mem := instL.size_zero_iff_forall_not_mem
+  size_erase_mem := instL.size_erase_mem
+
+local instance LawfulDMapLike_of_LawfulMapLike' {γ α β} [inst : MapLike γ α β]
+  [instL : LawfulMapLike γ α β] :
+  LawfulDMapLike (inst:=DMapLike_of_MapLike inst) γ α (fun _ => β) :=
+  LawfulDMapLike_of_LawfulMapLike (inst:=DMapLike_of_MapLike inst)
+
+theorem LawfulMapLike.mem_iff_getElem?_eq_some {γ α β} [inst : MapLike γ α β] [LawfulMapLike γ α β] {m : γ} {k : α} : k ∈ m ↔ ∃ v, m[k]? = .some v :=
+  LawfulDMapLike.mem_iff_dGetElem?_eq_some (inst:=DMapLike_of_MapLike inst)
+
+theorem LawfulMapLike.not_mem_iff_getElem?_eq_none {γ α β} [inst : MapLike γ α β] [LawfulMapLike γ α β] {m : γ} {k : α} : k ∉ m ↔ m[k]? = .none :=
+  LawfulDMapLike.not_mem_iff_dGetElem?_eq_none (inst:=DMapLike_of_MapLike inst)
+
+theorem LawfulMapLike.mem_insert {γ α β} [inst : MapLike γ α β] [LawfulMapLike γ α β] {m : γ} {k a : α} {v : β} :
+  a ∈ insert m k v ↔ (k = a) ∨ a ∈ m :=
+  LawfulDMapLike.mem_insert (inst:=DMapLike_of_MapLike inst)
+
+theorem LawfulMapLike.mem_erase {γ α β} [inst : MapLike γ α β] [LawfulMapLike γ α β] {m : γ} {k a : α} :
+  a ∈ erase (β:=β) m k ↔ k ≠ a ∧ a ∈ m :=
+  LawfulDMapLike.mem_erase (inst:=DMapLike_of_MapLike inst)
+
+open Classical in
+theorem LawfulMapLike.getElem?_eq_none_iff {γ α β} [inst : MapLike γ α β] [LawfulMapLike γ α β]
+  {c : γ} {i : α} : c[i]? = .none ↔ i ∉ c := by
+  simp only [getElem?_def]
+  split <;> simp_all
+
+theorem LawfulMapLike.getElem?_eq_some_getElem {γ α β} [inst : MapLike γ α β] [LawfulMapLike γ α β] {m : γ} {k : α} (h : k ∈ m) : m[k]? = .some m[k] :=
+  LawfulDMapLike.dGetElem?_eq_some_dGetElem (inst:=DMapLike_of_MapLike inst) h
+
+theorem LawfulMapLike.getElem!_eq_getElem {γ α β} [Inhabited β] [inst : MapLike γ α β] [LawfulMapLike γ α β] {m : γ} {k : α} (h : k ∈ m) :
+  m[k]! = m[k] := LawfulDMapLike.dGetElem!_eq_dGetElem (inst:=DMapLike_of_MapLike inst) h
+
+theorem LawfulMapLike.getElem!_eq_default {γ α β} [Inhabited β] [inst : MapLike γ α β] [LawfulMapLike γ α β] {m : γ} {k : α} (h : k ∉ m) :
+  m[k]! = default := LawfulDMapLike.dGetElem!_eq_default (inst:=DMapLike_of_MapLike inst) h
+
+theorem LawfulMapLike.getElem!_eq_get!_getElem? {γ α β} [Inhabited β] [inst : MapLike γ α β] [LawfulMapLike γ α β] {m : γ} {k : α} :
+  m[k]! = m[k]?.get! := LawfulDMapLike.dGetElem!_eq_get!_dGetElem? (inst:=DMapLike_of_MapLike inst)
+
+theorem LawfulMapLike.getElem?_eq_some_getElem! {γ α β} [Inhabited β] [inst : MapLike γ α β] [LawfulMapLike γ α β] {m : γ} {k : α} (h : k ∈ m) :
+  m[k]? = .some m[k]! := LawfulDMapLike.dGetElem?_eq_some_dGetElem! (inst:=DMapLike_of_MapLike inst) h
+
+theorem LawfulMapLike.getElem?_eq_none {γ α β} [Inhabited β]  [inst : MapLike γ α β] [LawfulMapLike γ α β] {m : γ} {k : α} (h : k ∉ m) :
+  m[k]? = .none := LawfulDMapLike.dGetElem?_eq_none (inst:=DMapLike_of_MapLike inst) h
+
+theorem LawfulMapLike.getElem_eq_iff_getElem?_eq_some {γ α β} [inst : MapLike γ α β] [LawfulMapLike γ α β] {m : γ} {k : α} {v : β} (h : k ∈ m) :
+  m[k] = v ↔ m[k]? = .some v := LawfulDMapLike.dGetElem_eq_iff_dGetElem?_eq_some (inst:=DMapLike_of_MapLike inst) h
+
+theorem LawfulMapLike.getElem_eq_of_getElem?_eq_some {γ α β} [inst : MapLike γ α β] [LawfulMapLike γ α β] {m : γ} {k : α} {v : β}
+  (h : m[k]? = .some v) : m[k]'(mem_iff_getElem?_eq_some.mpr ⟨_, h⟩) = v :=
+  LawfulDMapLike.dGetElem_eq_of_dGetElem?_eq_some (inst:=DMapLike_of_MapLike inst) h
+
+theorem LawfulMapLike.getElem_eq_getElem_iff_getElem?_eq_getElem? {γ α β} [inst : MapLike γ α β] [LawfulMapLike γ α β] {m₁ m₂ : γ} {k : α}
+  (h₁ : k ∈ m₁) (h₂ : k ∈ m₂) : m₁[k] = m₂[k] ↔ m₁[k]? = m₂[k]? :=
+  LawfulDMapLike.dGetElem_eq_dGetElem_iff_dGetElem?_eq_dGetElem? (inst:=DMapLike_of_MapLike inst) h₁ h₂
+
+theorem LawfulMapLike.getElem_insert_self {γ α β} [inst : MapLike γ α β] [LawfulMapLike γ α β] {m : γ} {k : α} {v : β} :
+  (insert m k v)[k]'(mem_insert.mpr (Or.inl rfl)) = v :=
+  LawfulDMapLike.dGetElem_insert_self (inst:=DMapLike_of_MapLike inst)
+
+theorem LawfulMapLike.getElem_insert_ne {γ α β} [inst : MapLike γ α β] [LawfulMapLike γ α β] {m : γ} {k a : α} {v : β} (h₁ : a ∈ insert m k v) (h₂ : k ≠ a) :
+  (insert m k v)[a] = m[a]'(Or.resolve_left (mem_insert.mp h₁) h₂) :=
+  LawfulDMapLike.dGetElem_insert_ne (inst:=DMapLike_of_MapLike inst) h₁ h₂
+
+theorem LawfulMapLike.getElem_erase {γ α β} [inst : MapLike γ α β] [LawfulMapLike γ α β] {m : γ} {k a : α} (h' : a ∈ erase m k) :
+  (erase (β:=β) m k)[a] = m[a]'((mem_erase.mp h').right) :=
+  LawfulDMapLike.dGetElem_erase (inst:=DMapLike_of_MapLike inst) h'
+
+theorem LawfulMapLike.insert_mem_keyEquiv {γ α β} [inst : MapLike γ α β] [LawfulMapLike γ α β]
+  {m : γ} {k : α} {v : β} (hmem : k ∈ m) : keyEquiv (α:=α) (β:=β) (insert (self:=inst) m k v) m :=
+  LawfulDMapLike.insert_mem_keyEquiv (inst:=DMapLike_of_MapLike inst) hmem
+
+theorem LawfulMapLike.erase_insert_not_mem_equiv {γ α β} [inst : MapLike γ α β] [LawfulMapLike γ α β]
+  {m : γ} {k : α} {v : β} (hnmem : k ∉ m) : equiv (α:=α) (β:=β) (erase (self:=inst) (insert (self:=inst) m k v) k) m :=
+  LawfulDMapLike.erase_insert_not_mem_equiv (inst:=DMapLike_of_MapLike inst) hnmem
+
+theorem LawfulMapLike.erase_not_mem_equiv {γ α β} [inst : MapLike γ α β] [LawfulMapLike γ α β]
+  {m : γ} {k : α} (hnmem : k ∉ m) : equiv (α:=α) (β:=β) (erase (self:=inst) m k) m :=
+  LawfulDMapLike.erase_not_mem_equiv (inst:=DMapLike_of_MapLike inst) hnmem
+
+theorem LawfulMapLike.insert_erase_mem_keyEquiv {γ α β} [inst : MapLike γ α β] [LawfulMapLike γ α β]
+  {m : γ} {k : α} {v : β} (hmem : k ∈ m) : keyEquiv (α:=α) (β:=β) (insert (erase (self:=inst) m k) k v) m :=
+  LawfulDMapLike.insert_erase_mem_keyEquiv (inst:=DMapLike_of_MapLike inst) hmem
+
+theorem LawfulMapLike.insert_erase_getElem_eq_equiv {γ α β} [inst : MapLike γ α β] [LawfulMapLike γ α β]
+  {m : γ} {k : α} {v : β} (hmem : k ∈ m) (hget : m[k] = v) : equiv (α:=α) (β:=β) (insert (erase (self:=inst) m k) k v) m :=
+  LawfulDMapLike.insert_erase_dGetElem_eq_equiv (inst:=DMapLike_of_MapLike inst) hmem hget
+
+theorem LawfulMapLike.exists_key_list {γ α β} [inst : MapLike γ α β] [LawfulMapLike γ α β] {m : γ} :
+  ∃ (l : List α), l.length = Size.size m ∧ l.Nodup ∧ ∀ k, k ∈ m ↔ k ∈ l :=
+  LawfulDMapLike.exists_key_list (inst:=DMapLike_of_MapLike inst)
+
+noncomputable def LawfulMapLike.exKeyList {γ α β} [inst : MapLike γ α β] [LawfulMapLike γ α β] (m : γ) : List α :=
+  (exists_key_list (α:=α) (β:=β) (m:=m)).choose
+
+noncomputable def LawfulMapLike.length_exKeyList_eq_size {γ α β} [inst : MapLike γ α β] [LawfulMapLike γ α β] {m : γ} :
+  (exKeyList (α:=α) (β:=β) m).length = Size.size m :=
+  (Exists.choose_spec exists_key_list).left
+
+noncomputable def LawfulMapLike.length_exKeyList_nodup {γ α β} [inst : MapLike γ α β] [LawfulMapLike γ α β] {m : γ} :
+  (exKeyList (α:=α) (β:=β) m).Nodup :=
+  (Exists.choose_spec exists_key_list).right.left
+
+noncomputable def LawfulMapLike.length_exKeyList_equiv {γ α β} [inst : MapLike γ α β] [LawfulMapLike γ α β] {m : γ} :
+  ∀ k, k ∈ m ↔ k ∈ (exKeyList (α:=α) (β:=β) m) :=
+  (Exists.choose_spec exists_key_list).right.right
+
+theorem LawfulMapLike.size_le_of_keySubset {γ₁ γ₂ α β} [inst₁ : MapLike γ₁ α β] [inst₂ : MapLike γ₂ α β]
+  [LawfulMapLike γ₁ α β] [LawfulMapLike γ₂ α β] {m₁ : γ₁} {m₂ : γ₂}
+  (hsub : keySubset (α:=α) (β:=β) m₁ m₂) : Size.size m₁ ≤ Size.size m₂ :=
+  LawfulDMapLike.size_le_of_keySubset (inst₁:=DMapLike_of_MapLike inst₁) (inst₂:=DMapLike_of_MapLike inst₂) hsub
+
+theorem LawfulMapLike.size_eq_of_keyEquiv {γ₁ γ₂ α β} [inst₁ : MapLike γ₁ α β] [inst₂ : MapLike γ₂ α β]
+  [LawfulMapLike γ₁ α β] [LawfulMapLike γ₂ α β] {m₁ : γ₁} {m₂ : γ₂}
+  (hequiv : keyEquiv (α:=α) (β:=β) m₁ m₂) : Size.size m₁ = Size.size m₂ :=
+  LawfulDMapLike.size_eq_of_keyEquiv (inst₁:=DMapLike_of_MapLike inst₁) (inst₂:=DMapLike_of_MapLike inst₂) hequiv
+
+theorem LawfulMapLike.keyEquiv_iff_size_eq_and_keySubset {γ₁ γ₂ α β} [inst₁ : MapLike γ₁ α β] [inst₂ : MapLike γ₂ α β]
+  [LawfulMapLike γ₁ α β] [LawfulMapLike γ₂ α β] {m₁ : γ₁} {m₂ : γ₂} :
+  keyEquiv (α:=α) (β:=β) m₁ m₂ ↔ Size.size m₁ = Size.size m₂ ∧ keySubset (α:=α) (β:=β) m₁ m₂ :=
+  LawfulDMapLike.keyEquiv_iff_size_eq_and_keySubset (inst₁:=DMapLike_of_MapLike inst₁) (inst₂:=DMapLike_of_MapLike inst₂)
+
+theorem LawfulMapLike.size_insert_mem {γ α β} [inst : MapLike γ α β] [LawfulMapLike γ α β] {m : γ}
+  {k : α} {v : β} (hmem : k ∈ m) : Size.size (insert (self:=inst) m k v) = Size.size m :=
+  LawfulDMapLike.size_insert_mem (inst:=DMapLike_of_MapLike inst) hmem
+
+theorem LawfulMapLike.size_insert_not_mem {γ α β} [inst : MapLike γ α β] [LawfulMapLike γ α β] {m : γ}
+  {k : α} {v : β} (hnmem : k ∉ m) : Size.size (insert (self:=inst) m k v) = Size.size m + 1 :=
+  LawfulDMapLike.size_insert_not_mem (inst:=DMapLike_of_MapLike inst) hnmem
+
+theorem LawfulMapLike.size_insert_le {γ α β} [inst : MapLike γ α β] [LawfulMapLike γ α β] {m : γ}
+  {k : α} {v : β} : Size.size (insert m k v) ≤ Size.size m + 1 :=
+  LawfulDMapLike.size_insert_le (inst:=DMapLike_of_MapLike inst)
+
+theorem LawfulMapLike.le_size_insert {γ α β} [inst : MapLike γ α β] [LawfulMapLike γ α β] {m : γ}
+  {k : α} {v : β} : Size.size m ≤ Size.size (insert m k v) :=
+  LawfulDMapLike.le_size_insert (inst:=DMapLike_of_MapLike inst)
+
+theorem LawfulMapLike.size_insert_gt_zero {γ α β} [inst : MapLike γ α β] [LawfulMapLike γ α β] {m : γ}
+  {k : α} {v : β} : Size.size (insert m k v) > 0 :=
+  LawfulDMapLike.size_insert_gt_zero (inst:=DMapLike_of_MapLike inst)
+
+theorem LawfulMapLike.size_erase_not_mem {γ α β} [inst : MapLike γ α β] [LawfulMapLike γ α β] {m : γ}
+  {k : α} (hnm : k ∉ m) : Size.size (erase (β:=β) m k) = Size.size m :=
+  LawfulDMapLike.size_erase_not_mem (inst:=DMapLike_of_MapLike inst) hnm
+
+theorem LawfulMapLike.size_erase_le {γ α β} [inst : MapLike γ α β] [LawfulMapLike γ α β] {m : γ}
+  {k : α} : Size.size (erase (β:=β) m k) ≤ Size.size m :=
+  LawfulDMapLike.size_erase_le (inst:=DMapLike_of_MapLike inst)
+
+theorem LawfulMapLike.le_size_erase {γ α β} [inst : MapLike γ α β] [LawfulMapLike γ α β] {m : γ}
+  {k : α} : Size.size m ≤ Size.size (erase (β:=β) m k) + 1 :=
+  LawfulDMapLike.le_size_erase (inst:=DMapLike_of_MapLike inst)
+
+theorem LawfulMapLike.getElem?_empty {γ α β} [inst : MapLike γ α β] [LawfulMapLike γ α β]
+  {capacity : Nat} {k : α} : (emptyWithCapacity (self:=inst) capacity)[k]? = .none :=
+  LawfulDMapLike.dGetElem?_empty (inst:=DMapLike_of_MapLike inst)
+
+theorem LawfulMapLike.getElem?_insert {γ α β} [inst : MapLike γ α β]
+  [LawfulMapLike γ α β] [DecidableEq α] {m : γ} {k a : α} {v : β} :
+  (insert m k v)[a]? = if (k = a) then some v else m[a]? := by
+  have h := LawfulDMapLike.dGetElem?_insert (inst:=DMapLike_of_MapLike inst) (m:=m) (k:=k) (a:=a) (v:=v)
+  simp only [dGetElem?, DMapLike_of_MapLike] at h
+  rw [h]; split
+  case isTrue heq => cases heq <;> rfl
+  case isFalse => rfl
+
+theorem LawfulMapLike.getElem?_erase {γ α β} [inst : MapLike γ α β]
+  [LawfulMapLike γ α β] [DecidableEq α] {m : γ} {k a : α} :
+  (erase (self:=inst) m k)[a]? = if (k = a) then .none else m[a]? :=
+  LawfulDMapLike.dGetElem?_erase (inst:=DMapLike_of_MapLike inst)
+
+open Classical in
+theorem LawfulMapLike.getElem?_eq_none_iff_getElem?_eq_none_of_keyEquiv {γ₁ γ₂ α β}
+  [inst₁ : MapLike γ₁ α β] [inst₂ : MapLike γ₂ α β] [LawfulMapLike γ₁ α β] [LawfulMapLike γ₂ α β]
+  {m₁ : γ₁} {m₂ : γ₂} (hequiv : MapLike.keyEquiv (α:=α) (β:=β) m₁ m₂)
+  (k : α) : m₁[k]? = .none ↔ m₂[k]? = .none := by
+  simp [hequiv k]
+
+theorem LawfulMapLike.equiv_iff_equiv' {γ₁ γ₂ α β}
+  [inst₁ : MapLike γ₁ α β] [inst₂ : MapLike γ₂ α β] [LawfulMapLike γ₁ α β] [LawfulMapLike γ₂ α β]
+  {m₁ : γ₁} {m₂ : γ₂} :
+  MapLike.equiv (α:=α) (β:=β) m₁ m₂ ↔ MapLike.equiv' (α:=α) (β:=β) m₁ m₂ :=
+  LawfulDMapLike.equiv_iff_equiv' (inst₁:=DMapLike_of_MapLike inst₁) (inst₂:=DMapLike_of_MapLike inst₂)
+
+theorem LawfulMapLike.equiv_iff_subset {γ₁ γ₂ α β}
+  [inst₁ : MapLike γ₁ α β] [inst₂ : MapLike γ₂ α β] [LawfulMapLike γ₁ α β] [LawfulMapLike γ₂ α β]
+  {m₁ : γ₁} {m₂ : γ₂} : equiv (α:=α) (β:=β) m₁ m₂ ↔ subset (α:=α) (β:=β) m₁ m₂ ∧ subset (α:=α) (β:=β) m₂ m₁ := by
+  rw [LawfulMapLike.equiv_iff_equiv', MapLike.equiv'_iff_subset]
+
+theorem LawfulMapLike.keySubset_of_subset {γ₁ γ₂ α β}
+  [inst₁ : MapLike γ₁ α β] [inst₂ : MapLike γ₂ α β] [LawfulMapLike γ₁ α β] [LawfulMapLike γ₂ α β]
+  {m₁ : γ₁} {m₂ : γ₂} (h : subset (α:=α) (β:=β) m₁ m₂) : keySubset (α:=α) (β:=β) m₁ m₂ := by
+  simp only [subset] at h
+  intro x
+  simp only [mem_iff_isSome_getElem?]
+  have hx := h x
+  revert hx
+  cases m₁[x]? <;> grind
+
+theorem LawfulMapLike.mem_congr {γ₁ γ₂ α β} [inst₁ : MapLike γ₁ α β] [inst₂ : MapLike γ₂ α β]
+  {m₁ : γ₁} {m₂ : γ₂} (hequiv : equiv (α:=α) (β:=β) m₁ m₂) (x : α) : x ∈ m₁ ↔ x ∈ m₂ := hequiv.left _
+
+theorem LawfulMapLike.getElem?_congr {γ₁ γ₂ α β} [inst₁ : MapLike γ₁ α β] [inst₂ : MapLike γ₂ α β]
+  [LawfulMapLike γ₁ α β] [LawfulMapLike γ₂ α β] {m₁ : γ₁} {m₂ : γ₂}
+  (hequiv : equiv (α:=α) (β:=β) m₁ m₂) (x : α) : m₁[x]? = m₂[x]? :=
+  LawfulMapLike.equiv_iff_equiv'.mp hequiv _
+
+theorem LawfulMapLike.getElem_congr {γ₁ γ₂ α β} [inst₁ : MapLike γ₁ α β] [inst₂ : MapLike γ₂ α β]
+  [LawfulMapLike γ₁ α β] [LawfulMapLike γ₂ α β] {m₁ : γ₁} {m₂ : γ₂}
+  (hequiv : equiv (α:=α) (β:=β) m₁ m₂) (x : α) (h₁ : x ∈ m₁) (h₂ : x ∈ m₂) : m₁[x] = m₂[x] :=
+  LawfulDMapLike.dGetElem_congr (inst₁:=DMapLike_of_MapLike inst₁) (inst₂:=DMapLike_of_MapLike inst₂) hequiv x h₁ h₂
+
+theorem LawfulMapLike.getElem_congr' {γ₁ γ₂ α β} [inst₁ : MapLike γ₁ α β] [inst₂ : MapLike γ₂ α β]
+  [LawfulMapLike γ₁ α β] [LawfulMapLike γ₂ α β] {m₁ : γ₁} {m₂ : γ₂}
+  (hequiv : equiv (α:=α) (β:=β) m₁ m₂) (x : α) (h₁ : x ∈ m₁) : m₁[x] = m₂[x]'((hequiv.left _).mp h₁) :=
+  LawfulDMapLike.dGetElem_congr' (inst₁:=DMapLike_of_MapLike inst₁) (inst₂:=DMapLike_of_MapLike inst₂) hequiv x h₁
+
+theorem LawfulMapLike.getElem!_congr {γ₁ γ₂ α β} [Inhabited β] [inst₁ : MapLike γ₁ α β] [inst₂ : MapLike γ₂ α β]
+  [LawfulMapLike γ₁ α β] [LawfulMapLike γ₂ α β] {m₁ : γ₁} {m₂ : γ₂}
+  (hequiv : equiv (α:=α) (β:=β) m₁ m₂) (x : α) : m₁[x]! = m₂[x]! :=
+  LawfulDMapLike.dGetElem!_congr (inst₁:=DMapLike_of_MapLike inst₁) (inst₂:=DMapLike_of_MapLike inst₂) hequiv x
+
+theorem LawfulMapLike.emptyWithCapacity_congr {γ₁ γ₂ α β} [inst₁ : MapLike γ₁ α β] [inst₂ : MapLike γ₂ α β]
+  [LawfulMapLike γ₁ α β] [LawfulMapLike γ₂ α β] (capacity₁ capacity₂ : Nat) :
+  equiv (α:=α) (β:=β)
+    (emptyWithCapacity (self:=inst₁) capacity₁)
+    (emptyWithCapacity (self:=inst₂) capacity₂) :=
+  LawfulDMapLike.emptyWithCapacity_congr (inst₁:=DMapLike_of_MapLike inst₁) (inst₂:=DMapLike_of_MapLike inst₂) _ _
+
+theorem LawfulMapLike.insert_congr {γ₁ γ₂ α β} [inst₁ : MapLike γ₁ α β] [inst₂ : MapLike γ₂ α β]
+  [LawfulMapLike γ₁ α β] [LawfulMapLike γ₂ α β] {m₁ : γ₁} {m₂ : γ₂}
+  (hequiv : equiv (α:=α) (β:=β) m₁ m₂) (k : α) (v : β) :
+  equiv (α:=α) (β:=β) (insert m₁ k v) (insert m₂ k v) :=
+  LawfulDMapLike.insert_congr (inst₁:=DMapLike_of_MapLike inst₁) (inst₂:=DMapLike_of_MapLike inst₂) hequiv k v
+
+open Classical in
+theorem LawfulMapLike.erase_congr {γ₁ γ₂ α β} [inst₁ : MapLike γ₁ α β] [inst₂ : MapLike γ₂ α β]
+  [LawfulMapLike γ₁ α β] [LawfulMapLike γ₂ α β] {m₁ : γ₁} {m₂ : γ₂}
+  (hequiv : equiv (α:=α) (β:=β) m₁ m₂) (k : α) :
+  equiv (α:=α) (β:=β) (erase m₁ (self:=inst₁) k) (erase m₂ (self:=inst₂) k) :=
+  LawfulDMapLike.erase_congr (inst₁:=DMapLike_of_MapLike inst₁) (inst₂:=DMapLike_of_MapLike inst₂) hequiv k
+
+theorem LawfulMapLike.size_congr {γ₁ γ₂ α β} [inst₁ : MapLike γ₁ α β] [inst₂ : MapLike γ₂ α β]
+  [LawfulMapLike γ₁ α β] [LawfulMapLike γ₂ α β] {m₁ : γ₁} {m₂ : γ₂}
+  (hequiv : equiv (α:=α) (β:=β) m₁ m₂) : Size.size m₁ = Size.size m₂ :=
+  LawfulDMapLike.size_congr (inst₁:=DMapLike_of_MapLike inst₁) (inst₂:=DMapLike_of_MapLike inst₂) hequiv
+
+instance {α β} [BEq α] [Hashable α] : MapLike (HashMap α β) α β where
+  emptyWithCapacity capacity := HashMap.emptyWithCapacity (capacity:=capacity)
+  insert := HashMap.insert
+  erase := HashMap.erase
+  size := HashMap.size
+
+instance {α β} [BEq α] [Hashable α] [LawfulBEq α] : LawfulMapLike (HashMap α β) α β where
+  not_mem_empty := by intro k n; simp [MapLike.emptyWithCapacity]
+  mem_iff_isSome_getElem? := HashMap.mem_iff_isSome_getElem?
+  getElem?_insert_self := HashMap.getElem?_insert_self
+  getElem?_insert_ne := by
+    intro m k a v h
+    simp [MapLike.insert, HashMap.getElem?_insert, h]
+  getElem?_erase_self := HashMap.getElem?_erase_self
+  getElem?_erase_ne := by
+    intro m k a h
+    simp [MapLike.erase, HashMap.getElem?_erase, h]
+  size_erase_mem := HashMap.size_erase_mem
+
+instance {α} : MapLike (OptArr α) Nat α where
+  emptyWithCapacity capacity := OptArr.emptyWithCapacity capacity
+  insert := OptArr.insert
+  erase := OptArr.erase
+  size := OptArr.size
+
+instance {α} : LawfulMapLike (OptArr α) Nat α where
+  not_mem_empty := OptArr.not_mem_empty
+  mem_iff_isSome_getElem? := OptArr.mem_iff_isSome_getElem?
+  getElem?_insert_self := OptArr.getElem?_insert_self
+  getElem?_insert_ne := OptArr.getElem?_insert_ne
+  getElem?_erase_self := OptArr.getElem?_erase_self
+  getElem?_erase_ne := OptArr.getElem?_erase_ne
+  size_erase_mem := OptArr.size_erase_mem
+
+instance {α β} [Ord α] : MapLike (TreeMap α β) α β where
+  emptyWithCapacity _ := TreeMap.empty
+  insert := TreeMap.insert
+  erase := TreeMap.erase
+  size := TreeMap.size
+
+instance {α β} [Ord α] [LawfulEqOrd α] [TransOrd α] : LawfulMapLike (TreeMap α β) α β where
+  not_mem_empty := TreeMap.not_mem_emptyc
+  mem_iff_isSome_getElem? := TreeMap.mem_iff_isSome_getElem?
+  getElem?_insert_self := TreeMap.getElem?_insert_self
+  getElem?_insert_ne := by
+    intro m k a v hne
+    simp only [MapLike.insert, TreeMap.getElem?_insert]
+    rw [ite_cond_eq_false]
+    rw [LawfulEqOrd.compare_eq_iff_eq]
+    simp [hne]
+  getElem?_erase_self := TreeMap.getElem?_erase_self
+  getElem?_erase_ne := by
+    intro m k a hne
+    simp only [MapLike.erase, TreeMap.getElem?_erase]
+    rw [ite_cond_eq_false]
+    rw [LawfulEqOrd.compare_eq_iff_eq]
+    simp [hne]
+  size_erase_mem := TreeMap.size_erase_mem
+
+instance {α β} [BEq α] [Hashable α] [EquivBEq α] [LawfulHashable α] : MapLike (ExtHashMap α β) α β where
+  emptyWithCapacity capacity := ExtHashMap.emptyWithCapacity capacity
+  insert := ExtHashMap.insert
+  erase := ExtHashMap.erase
+  size := ExtHashMap.size
+
+instance {α β} [BEq α] [Hashable α] [LawfulBEq α] [LawfulHashable α] : LawfulMapLike (ExtHashMap α β) α β where
+  not_mem_empty := by intro k n; simp [MapLike.emptyWithCapacity]
+  mem_iff_isSome_getElem? := ExtHashMap.mem_iff_isSome_getElem?
+  getElem?_insert_self := ExtHashMap.getElem?_insert_self
+  getElem?_insert_ne := by
+    intros m k a v hne
+    simp [MapLike.insert, ExtHashMap.getElem?_insert, hne]
+  getElem?_erase_self := ExtHashMap.getElem?_erase_self
+  getElem?_erase_ne := by
+    intros m k a hne
+    simp [MapLike.erase, ExtHashMap.getElem?_erase, hne]
+  size_erase_mem := Std.ExtHashMap.size_erase_mem
+
+instance {α β} [Ord α] [TransOrd α] : MapLike (ExtTreeMap α β) α β where
+  emptyWithCapacity _ := ExtTreeMap.empty
+  insert := ExtTreeMap.insert
+  erase := ExtTreeMap.erase
+  size := ExtTreeMap.size
+
+instance {α β} [Ord α] [LawfulEqOrd α] [TransOrd α] : LawfulMapLike (ExtTreeMap α β) α β where
+  not_mem_empty := TreeMap.not_mem_emptyc
+  mem_iff_isSome_getElem? := ExtTreeMap.mem_iff_isSome_getElem?
+  getElem?_insert_self := ExtTreeMap.getElem?_insert_self
+  getElem?_insert_ne := by
+    intro m k a v hne
+    simp only [MapLike.insert, ExtTreeMap.getElem?_insert]
+    rw [ite_cond_eq_false]
+    rw [LawfulEqOrd.compare_eq_iff_eq]
+    simp [hne]
+  getElem?_erase_self := ExtTreeMap.getElem?_erase_self
+  getElem?_erase_ne := by
+    intro m k a hne
+    simp only [MapLike.erase, ExtTreeMap.getElem?_erase]
+    rw [ite_cond_eq_false]
+    rw [LawfulEqOrd.compare_eq_iff_eq]
+    simp [hne]
+  size_erase_mem := ExtTreeMap.size_erase_mem
+
+end MapLike
