ADT/Size.lean
@@ -1,0 +1,152 @@
+/-
+Copyright (c) 2025 Amazon.com, Inc. or its affiliates. All Rights Reserved.
+Released under Apache 2.0 license as described in the file LICENSE.
+Authors: Yicheng Qian
+-/
+
+import Lean
+import ADT.OptArr
+import ADT.Lemmas
+import Std.Data
+open Std
+
+class Size (γ : Type u) where
+  size : γ → Nat
+
+instance {α} : Size (Option α) where
+  size o := match o with | .some _ => 1 | .none => 0
+
+instance {α} : Size (List α) where
+  size := List.length
+
+instance {α} : Size (Array α) where
+  size := Array.size
+
+instance {α β} [BEq α] [Hashable α] : Size (DHashMap α β) where
+  size := DHashMap.size
+
+instance {α β} [Ord α] : Size (DTreeMap α β) where
+  size := DTreeMap.size
+
+instance {α β} [BEq α] [Hashable α] [EquivBEq α] [LawfulHashable α] : Size (ExtDHashMap α β) where
+  size := ExtDHashMap.size
+
+instance {α β} [Ord α] : Size (ExtDTreeMap α β) where
+  size := ExtDTreeMap.size
+
+instance {α β} [BEq α] [Hashable α] : Size (HashMap α β) where
+  size := HashMap.size
+
+instance {α} : Size (OptArr α) where
+  size := OptArr.size
+
+instance {α β} [Ord α] : Size (TreeMap α β) where
+  size := TreeMap.size
+
+instance {α β} [BEq α] [Hashable α] [EquivBEq α] [LawfulHashable α] : Size (ExtHashMap α β) where
+  size := ExtHashMap.size
+
+instance {α β} [Ord α] : Size (ExtTreeMap α β) where
+  size := ExtTreeMap.size
+
+instance {α} [BEq α] [Hashable α] : Size (HashSet α) where
+  size := HashSet.size
+
+instance {α} [Ord α] : Size (TreeSet α) where
+  size := TreeSet.size
+
+instance {α} [BEq α] [Hashable α] [EquivBEq α] [LawfulHashable α] : Size (ExtHashSet α) where
+  size := ExtHashSet.size
+
+instance {α} [Ord α] : Size (ExtTreeSet α) where
+  size := ExtTreeSet.size
+
+class LawfulMemSize (γ : Type u) (α : Type v) [Size γ] [Membership α γ] where
+  size_zero_iff_forall_not_mem : ∀ {m : γ}, Size.size m = 0 ↔ ∀ (x : α), ¬ x ∈ m
+
+theorem LawfulMemSize.size_ne_zero_iff_exists_mem {γ α} [Size γ] [Membership α γ] [LawfulMemSize γ α] {m : γ} :
+  Size.size m ≠ 0 ↔ ∃ (x : α), x ∈ m := by
+  rw [ne_eq, size_zero_iff_forall_not_mem (α:=α)]; simp
+
+theorem LawfulMemSize.size_gt_zero_iff_exists_mem {γ α} [Size γ] [Membership α γ] [LawfulMemSize γ α] {m : γ} :
+  Size.size m > 0 ↔ ∃ (x : α), x ∈ m := by
+  rw [← size_ne_zero_iff_exists_mem, Nat.ne_zero_iff_zero_lt];
+
+instance {α} : LawfulMemSize (Option α) α where
+  size_zero_iff_forall_not_mem := by
+    intro m; cases m <;> simp [Size.size]
+
+instance {α} : LawfulMemSize (List α) α where
+  size_zero_iff_forall_not_mem := by
+    intro m
+    simp only [Size.size, List.length_eq_zero_iff, List.eq_nil_iff_forall_not_mem]
+
+instance {α} : LawfulMemSize (Array α) α where
+  size_zero_iff_forall_not_mem := by
+    intro m
+    simp only [Size.size, Array.size_eq_zero_iff, Array.eq_empty_iff_forall_not_mem]
+
+instance {α β} [BEq α] [Hashable α] [EquivBEq α] [LawfulHashable α] : LawfulMemSize (DHashMap α β) α where
+  size_zero_iff_forall_not_mem := DHashMap.size_zero_iff_forall_not_mem
+
+instance {α β} [Ord α] [TransOrd α] : LawfulMemSize (DTreeMap α β) α where
+  size_zero_iff_forall_not_mem := by
+    intro m
+    rw [← DTreeMap.isEmpty_iff_forall_not_mem,
+        DTreeMap.isEmpty_eq_size_eq_zero]
+    simp [Size.size]
+
+instance {α β} [BEq α] [Hashable α] [EquivBEq α] [LawfulHashable α] : LawfulMemSize (ExtDHashMap α β) α where
+  size_zero_iff_forall_not_mem := by
+    intro m
+    rw [← ExtDHashMap.eq_empty_iff_forall_not_mem,
+        ExtDHashMap.eq_empty_iff_size_eq_zero]
+    rfl
+
+instance {α β} [Ord α] [TransOrd α] : LawfulMemSize (ExtDTreeMap α β) α where
+  size_zero_iff_forall_not_mem := by
+    intro m
+    rw [← ExtDTreeMap.isEmpty_iff_forall_not_mem,
+        ExtDTreeMap.isEmpty_eq_size_eq_zero]
+    simp [Size.size]
+
+instance {α β} [BEq α] [Hashable α] [EquivBEq α] [LawfulHashable α] : LawfulMemSize (HashMap α β) α where
+  size_zero_iff_forall_not_mem := by
+    intro m; simp only [Size.size]
+    apply HashMap.size_zero_iff_forall_not_mem
+
+instance {α} : LawfulMemSize (OptArr α) Nat where
+  size_zero_iff_forall_not_mem := OptArr.size_zero_iff_forall_not_mem
+
+instance {α β} [Ord α] [TransOrd α] : LawfulMemSize (TreeMap α β) α where
+  size_zero_iff_forall_not_mem := by
+    intro m
+    rw [← TreeMap.isEmpty_iff_forall_not_mem,
+        TreeMap.isEmpty_eq_size_eq_zero]
+    simp [Size.size]
+
+instance {α β} [BEq α] [Hashable α] [EquivBEq α] [LawfulHashable α] : LawfulMemSize (ExtHashMap α β) α where
+  size_zero_iff_forall_not_mem := by
+    intro m
+    rw [← ExtHashMap.eq_empty_iff_forall_not_mem,
+        ExtHashMap.eq_empty_iff_size_eq_zero]
+    rfl
+
+instance {α β} [Ord α] [TransOrd α] : LawfulMemSize (ExtTreeMap α β) α where
+  size_zero_iff_forall_not_mem := by
+    intro m
+    rw [← ExtTreeMap.isEmpty_iff_forall_not_mem,
+        ExtTreeMap.isEmpty_eq_size_eq_zero]
+    simp [Size.size]
+
+instance {α} [BEq α] [Hashable α] [EquivBEq α] [LawfulHashable α] : LawfulMemSize (HashSet α) α where
+  size_zero_iff_forall_not_mem := HashSet.size_zero_iff_forall_not_mem
+
+instance {α} [Ord α] [TransOrd α] : LawfulMemSize (TreeSet α) α where
+  size_zero_iff_forall_not_mem := TreeSet.size_zero_iff_forall_not_mem
+
+instance {α} [BEq α] [Hashable α] [EquivBEq α] [LawfulHashable α] : LawfulMemSize (ExtHashSet α) α where
+  size_zero_iff_forall_not_mem := ExtHashSet.size_zero_iff_forall_not_mem
+
+instance {α} [Ord α] [TransOrd α] : LawfulMemSize (ExtTreeSet α) α where
+  size_zero_iff_forall_not_mem := ExtTreeSet.size_zero_iff_forall_not_mem
